fix definitions for udivB sdivB

src/BBUdiv.v
@@ -39,21 +39,30 @@ Fixpoint udivB_rec (n m : bits) i : bits * bits :=
     (qi, ri)
   end.
   
-Definition udivB (n m : bits) := udivB_rec n m (act_size n - (act_size m) + 1).
+Definition udivB (n m : bits) :=
+  if (m == zeros (size m)) then (zeros (size n), zeros (size n))
+  else  udivB_rec n m (act_size n - (act_size m) + 1).
 
-Eval compute in (to_nat (udivB (from_nat 8 185) (from_nat 4 13)).1).
+(*Eval compute in (to_nat (udivB (from_nat 8 185) (from_nat 4 13)).1).
 Eval compute in (to_nat (udivB (from_nat 8 185) (from_nat 4 13)).2).
-
 Eval compute in (to_nat (udivB (from_nat 15 15) (from_nat 3 2)).1).
 Eval compute in (to_nat (udivB (from_nat 15 15) (from_nat 3 2)).2).
+ *)
 
-
-
+Lemma udivB_to_nat : forall p q, size p = size q -> (udivB p q).1 = from_nat (size p) (div.divn (to_nat p) (to_nat q)).
+Proof.
+  elim =>[|phd ptl IH] q /= Hsz.
+  symmetry in Hsz; by rewrite  (size0nil Hsz)/=.
+  rewrite /udivB/=.
+  case Hq0: (q == zeros (size q)).
+Admitted.  
+  
+  
 Fixpoint bit_blast_udiv_rec g ls1 ls2 i : generator * cnf * word * word :=
   match i with
   | 0 => let '(g_shr, cs_shr, lrs_shr) := bit_blast_ashr_int g ls1 (act_sizel ls1 - act_sizel ls2 +1) in (g_shr, cs_shr, (copy (size ls1) lit_ff), lrs_shr)
   | S i' =>
-    let ai := nth lit_ff ls1 (act_sizel ls1 - act_sizel ls2 +1 ) in
+    let ai := nth lit_ff ls1 (act_sizel ls1 - i' - act_sizel ls2 +1 ) in
     let '(g_udiv, cs_udiv, q_udiv, r_udiv) := bit_blast_udiv_rec g ls1 ls2 i' in
     let di := dropmsl (joinlsl ai r_udiv) in
     let '(g_ge, cs_ge, lrs_ge) := bit_blast_uge g_udiv di ls2 in
@@ -65,4 +74,49 @@ Fixpoint bit_blast_udiv_rec g ls1 ls2 i : generator * cnf * word * word :=
   end.
 
 Definition bit_blast_udiv g ls1 ls2 := bit_blast_udiv_rec g ls1 ls2 (act_sizel ls1 -act_sizel ls2 +1).
+
+Fixpoint mk_env_udiv_rec E g ls1 ls2 i : env * generator * cnf * word * word :=
+  match i with
+  | 0 => let '(E_shr, g_shr, cs_shr, lrs_shr) := mk_env_ashr_int E g ls1 (act_sizel ls1 - act_sizel ls2 +1) in (E_shr, g_shr, cs_shr, (copy (size ls1) lit_ff), lrs_shr)
+  | S i' =>
+    let ai := nth lit_ff ls1 (act_sizel ls1 - i' - act_sizel ls2 +1 ) in
+    let '(E_udiv, g_udiv, cs_udiv, q_udiv, r_udiv) := mk_env_udiv_rec E g ls1 ls2 i' in
+    let di := dropmsl (joinlsl ai r_udiv) in
+    let '(E_ge, g_ge, cs_ge, lrs_ge) := mk_env_uge E g_udiv di ls2 in
+    let qi := dropmsl (joinlsl lrs_ge q_udiv) in
+    if (lrs_ge==lit_tt) then
+      let '(E_sub, g_sub, cs_sub, lrs_sub) := mk_env_sub E g_ge di ls2 in
+      (E_sub, g_sub, catrev (catrev cs_udiv cs_ge) cs_sub, qi, lrs_sub)
+    else (E_ge, g_ge, catrev cs_udiv cs_ge, qi, di)
+  end.
+
+Definition mk_env_udiv E g ls1 ls2 := mk_env_udiv_rec E g ls1 ls2 (act_sizel ls1 -act_sizel ls2 +1).
+
+Lemma bit_blast_udiv_rec_correct g ls1 ls2 i g' cs qlrs rlrs E bs1 bs2 :
+  bit_blast_udiv_rec g ls1 ls2 i = (g', cs, qlrs, rlrs) ->
+  enc_bits E ls1 bs1 ->
+  enc_bits E ls2 bs2 ->
+  interp_cnf E (add_prelude cs) ->
+  enc_bits E qlrs (udivB_rec bs1 bs2 i).1 ->
+  enc_bits E rlrs (udivB_rec bs1 bs2 i).2.
+Proof.
+Admitted.
+
+
+Lemma bit_blast_udiv_correct g ls1 ls2 g' cs qlrs rlrs E bs1 bs2 :
+  bit_blast_udiv g ls1 ls2 = (g', cs, qlrs, rlrs) ->
+  enc_bits E ls1 bs1 ->
+  enc_bits E ls2 bs2 ->
+  interp_cnf E (add_prelude cs) ->
+  enc_bits E qlrs (udivB bs1 bs2).1 ->
+  enc_bits E rlrs (udivB bs1 bs2).2.
+Proof.
+Admitted.
+
+
+Lemma mk_env_udiv_rec_is_bit_blast_udiv_rec E g ls1 ls2 i g' cs qlrs rlrs E' :
+  mk_env_udiv_rec E g ls1 ls2 i = (E', g', cs, qlrs, rlrs) ->
+  bit_blast_udiv_rec g ls1 ls2 i = (g', cs, qlrs, rlrs).
+Proof.
+Admitted.
 
